Prover termination of conflict rule

Simple_Clause_Learning/Termination.thy
@@ -7,28 +7,120 @@ begin
 section \<open>Extra Lemmas\<close>
 
 
+subsection \<open>Prod_Extra\<close>
+
+definition lex_prodp where
+  "lex_prodp RA RB x y \<longleftrightarrow> RA (fst x) (fst y) \<or> fst x = fst y \<and> RB (snd x) (snd y)"
+
+lemma lex_prod_lex_prodp_eq:
+  "lex_prod {(x, y). RA x y} {(x, y). RB x y} = {(x, y). lex_prodp RA RB x y}"
+  unfolding lex_prodp_def lex_prod_def
+  by auto
+
+lemma reflp_on_lex_prodp:
+  assumes "reflp_on A RA"
+  shows "reflp_on (A \<times> B) (lex_prodp RA RB)"
+proof (rule reflp_onI)
+  fix x assume "x \<in> A \<times> B"
+  hence "fst x \<in> A"
+    by auto
+  thus "lex_prodp RA RB x x"
+    by (simp add: lex_prodp_def \<open>reflp_on A RA\<close>[THEN reflp_onD])
+qed
+
+lemma transp_lex_prodp:
+  assumes "transp RA" and "transp RB"
+  shows "transp (lex_prodp RA RB)"
+proof (rule transpI)
+  fix x y z assume "lex_prodp RA RB x y" and "lex_prodp RA RB y z"
+  thus "lex_prodp RA RB x z"
+    by (auto simp add: lex_prodp_def \<open>transp RA\<close>[THEN transpD, of "fst x" "fst y" "fst z"]
+        \<open>transp RB\<close>[THEN transpD, of "snd x" "snd y" "snd z"])
+qed
+
+lemma asymp_lex_prodp:
+  assumes "asymp RA" and "asymp RB"
+  shows "asymp (lex_prodp RA RB)"
+proof (rule asympI)
+  fix x y assume "lex_prodp RA RB x y"
+  thus "\<not> lex_prodp RA RB y x"
+    using assms by (metis (full_types, opaque_lifting) asymp.cases lex_prodp_def)
+qed
+
+lemma totalp_on_lex_prodp:
+  assumes "totalp_on A RA" and "totalp_on B RB"
+  shows "totalp_on (A \<times> B) (lex_prodp RA RB)"
+proof (rule totalp_onI)
+  fix x y assume "x \<in> A \<times> B" and "y \<in> A \<times> B" and "x \<noteq> y"
+  then show "lex_prodp RA RB x y \<or> lex_prodp RA RB y x"
+    using assms
+    by (metis (full_types) lex_prodp_def mem_Times_iff prod_eq_iff totalp_on_def)
+qed
+
+lemma wfP_lex_prodp:
+  assumes "wfP RA" and "wfP RB"
+  shows "wfP (lex_prodp RA RB)"
+  using assms
+  by (rule wf_lex_prod[of "{(x, y). RA x y}" "{(x, y). RB x y}", unfolded lex_prod_lex_prodp_eq, to_pred])
+  
+
+instantiation prod :: (preorder, preorder) order begin
+
+definition less_prod :: "'a \<times> 'b \<Rightarrow> 'a \<times> 'b \<Rightarrow> bool" where
+  "x < y \<longleftrightarrow> lex_prodp less less x y"
+
+definition less_eq_prod :: "'a \<times> 'b \<Rightarrow> 'a \<times> 'b \<Rightarrow> bool" where
+  "less_eq_prod x y \<longleftrightarrow> x < y \<or> x = y"
+
+instance
+proof intro_classes
+  fix x y :: "'a \<times> 'b"
+  show "(x < y) = (x \<le> y \<and> \<not> y \<le> x)"
+    unfolding less_eq_prod_def less_prod_def
+    using order_less_imp_not_less
+    by (metis (full_types, opaque_lifting) lex_prodp_def order_less_imp_not_less)
+next
+  fix x :: "'a \<times> 'b"
+  show "x \<le> x"
+    unfolding less_eq_prod_def
+    by simp
+next
+  fix x y z :: "'a \<times> 'b"
+  show "x \<le> y \<Longrightarrow> y \<le> z \<Longrightarrow> x \<le> z"
+    unfolding less_eq_prod_def less_prod_def
+    using transp_lex_prodp[OF transp_less transp_less, THEN transpD]
+    by metis
+next
+  fix x y :: "'a \<times> 'b"
+  show "x \<le> y \<Longrightarrow> y \<le> x \<Longrightarrow> x = y"
+    unfolding less_eq_prod_def less_prod_def
+    using asymp_lex_prodp[OF asymp_less asymp_less, THEN asympD]
+    by metis
+qed
+
+end
+
+instance prod :: (linorder, linorder) linorder
+proof intro_classes
+  fix x y :: "'a \<times> 'b"
+  show "x \<le> y \<or> y \<le> x"
+    unfolding less_eq_prod_def less_prod_def
+    using totalp_on_lex_prodp[OF totalp_less totalp_less, of UNIV UNIV, simplified, THEN totalpD]
+    by metis
+qed
+
+instance prod :: (wellorder, wellorder) wellorder
+proof intro_classes
+  fix P :: "'a \<times> 'b \<Rightarrow> bool" and x :: "'a \<times> 'b"
+  assume "\<And>x. (\<And>y. y < x \<Longrightarrow> P y) \<Longrightarrow> P x"
+  then show "P x"
+    unfolding less_prod_def
+    using wfP_lex_prodp[OF wfP_less wfP_less, THEN wfP_induct]
+    by metis
+qed
+
+
 subsection \<open>Wellfounded_Extra\<close>
-
-lemma wf_if_measurable:
-  fixes f :: "'a \<Rightarrow> 'b" and s :: "('b \<times> 'b) set"
-  assumes
-    "wf s"
-    "\<And>x y. (x, y) \<in> r \<Longrightarrow> (f x, f y) \<in> s"
-  shows "wf r"
-  by (metis assms in_inv_image wfE_min wfI_min wf_inv_image)
-
-lemma wfP_if_measurable:
-  fixes f :: "'a \<Rightarrow> 'b" and R :: "'a \<Rightarrow> 'a \<Rightarrow> bool" and S :: "'b \<Rightarrow> 'b \<Rightarrow> bool"
-  assumes
-    "wfP S"
-    "\<And>x y. R x y \<Longrightarrow> S (f x) (f y)"
-  shows "wfP R"
-  using assms wf_if_measurable[to_pred, of S R f] by simp
-
-lemma wfP_if_measurable_as_nat:
-  fixes f :: "_ \<Rightarrow> nat"
-  shows "(\<And>x y. R x y \<Longrightarrow> f x < f y) \<Longrightarrow> wfP R"
-  by (rule wfP_if_measurable[of "(<) :: nat \<Rightarrow> nat \<Rightarrow> bool", simplified])
 
 lemma wf_union_if_measurable:
   fixes
@@ -41,7 +133,7 @@ lemma wf_union_if_measurable:
     "\<And>x y. (x, y) \<in> S \<Longrightarrow> (f x, f y) \<in> Q"
     "\<And>x y. (x, y) \<in> R \<Longrightarrow> (f x, f y) \<in> Q \<or> f x = f y"
   shows "wf (R \<union> S)"
-proof (rule wf_if_measurable)
+proof (rule wf_if_convertible_to_wf)
   show "wf (Q <*lex*> T)"
     by (rule wf_lex_prod[OF \<open>wf Q\<close> \<open>wf T\<close>])
 next
@@ -76,6 +168,12 @@ proof -
 qed
 
 
+subsection \<open>FSet_Extra\<close>
+
+lemma finsert_Abs_fset: "finite A \<Longrightarrow> finsert a (Abs_fset A) = Abs_fset (insert a A)"
+  by (simp add: eq_onp_same_args finsert.abs_eq)
+
+
 section \<open>Termination\<close>
 
 context scl begin
@@ -83,9 +181,26 @@ context scl begin
 definition ground_lits_of_lit where
   "ground_lits_of_lit L = {L \<cdot>l \<gamma> | \<gamma> . is_ground_lit (L \<cdot>l \<gamma>)}"
 
-fun \<M> :: "_ \<Rightarrow> _ \<Rightarrow> ('f, 'v) state \<Rightarrow> ('f, 'v) Term.term literal set" where
+(* fun \<M> :: "_ \<Rightarrow> _ \<Rightarrow> ('f, 'v) state \<Rightarrow> ('f, 'v) Term.term literal set" where
   "\<M> N \<beta> (\<Gamma>, U, D) =
-    {L \<in> \<Union>(ground_lits_of_lit ` \<Union>(set_mset ` fset N)). atm_of L \<prec>\<^sub>B \<beta>} - fst ` set \<Gamma>"
+    {L \<in> \<Union>(ground_lits_of_lit ` \<Union>(set_mset ` fset N)). atm_of L \<prec>\<^sub>B \<beta>} - fst ` set \<Gamma>" *)
+
+definition \<M>_prop_deci :: "_ \<Rightarrow> _ \<Rightarrow> (_, _) Term.term literal fset" where
+  "\<M>_prop_deci \<beta> \<Gamma> = Abs_fset {L. atm_of L \<prec>\<^sub>B \<beta> \<or> atm_of L = \<beta>} |-| (fst |`| fset_of_list \<Gamma>)"
+
+primrec \<M>_skip_fact_reso where
+  "\<M>_skip_fact_reso [] C = []" |
+  "\<M>_skip_fact_reso (Lc # \<Gamma>) C = count C (fst Lc) # \<M>_skip_fact_reso \<Gamma> C"
+
+definition \<M> :: "_ \<Rightarrow> _ \<Rightarrow> ('f, 'v) state \<Rightarrow> ('f, 'v) Term.term literal fset \<times> nat list" where
+  "\<M> N \<beta> S =
+    (case state_conflict S of
+      None \<Rightarrow> (\<M>_prop_deci \<beta> (state_trail S), [])
+    | Some (C, \<gamma>) \<Rightarrow> ({||}, \<M>_skip_fact_reso (state_trail S) (C \<cdot> \<gamma>)))"
+
+term "lex_prodp (|\<subset>|) (List.lexordp (<))"
+term "List.lexordp (<)"
+find_consts "nat \<Rightarrow> nat \<Rightarrow> bool"
 
 lemma minus_psubset_minusI:
   assumes "C \<subset> B" and "B \<subseteq> A"
@@ -98,6 +213,20 @@ next
     using assms by blast
 qed
 
+lemma minus_pfsubset_minusI:
+  assumes "C |\<subset>| B" and "B |\<subseteq>| A"
+  shows "(A |-| B |\<subset>| A |-| C)"
+proof (rule FSet.pfsubsetI)
+  show "A |-| B |\<subseteq>| A |-| C"
+    using assms(1) by blast
+next
+  show "A |-| B \<noteq> A |-| C"
+    using assms by blast
+qed
+
+lemma Abs_fset_minus: "finite A \<Longrightarrow> finite B \<Longrightarrow> Abs_fset (A - B) = Abs_fset A |-| Abs_fset B"
+  by (metis Abs_fset_inverse fset_inverse mem_Collect_eq minus_fset)
+
 lemma
   fixes N \<beta>
   defines
@@ -106,7 +235,7 @@ lemma
     "invars \<equiv> \<lambda>S _. trail_atoms_lt \<beta> S \<and> trail_lits_ground S \<and> trail_lits_from_clauses N S \<and>
       initial_lits_generalize_learned_trail_conflict N S"
   shows "wfP (scl_without_backtrack \<sqinter> invars)\<inverse>\<inverse>"
-proof (rule wfP_if_measurable)
+proof (rule wfP_if_convertible_to_wfP)
   fix S S' :: "('f, 'v) state"
   assume "(scl_without_backtrack \<sqinter> invars)\<inverse>\<inverse> S S'"
   hence step: "scl_without_backtrack S' S" and invars: "invars S' S"
@@ -133,47 +262,45 @@ proof (rule wfP_if_measurable)
     using \<open>trail_lits_from_clauses N S\<close> \<open>initial_lits_generalize_learned_trail_conflict N S\<close>
     by (simp add: trail_lits_from_init_clausesI)
 
-  from step show "(\<M> N \<beta> S) < (\<M> N \<beta> S')"
+  let ?less = "lex_prodp (|\<subset>|) (\<lambda>x y. (x, y) \<in> List.lenlex {(x, y). x < y})"
+
+  from step show "?less (\<M> N \<beta> S) (\<M> N \<beta> S')"
     unfolding scl_without_backtrack_def sup_apply sup_bool_def
   proof (elim disjE)
     assume "decide N \<beta> S' S"
-    thus "(\<M> N \<beta> S) < (\<M> N \<beta> S')"
+    thus "?less (\<M> N \<beta> S) (\<M> N \<beta> S')"
     proof (cases N \<beta> S' S rule: decide.cases)
       case (decideI L \<gamma> \<Gamma> U)
-      show ?thesis
-        unfolding decideI(1,2) trail_decide_def \<M>.simps
-      proof (rule minus_psubset_minusI)
-        show "fst ` set \<Gamma> \<subset> fst ` set ((L \<cdot>l \<gamma>, None) # \<Gamma>)"
-          using decideI
-          by (auto simp add: trail_decide_def trail_defined_lit_def)
+      have "\<M>_prop_deci \<beta> ((L \<cdot>l \<gamma>, None) # \<Gamma>) |\<subset>| \<M>_prop_deci \<beta> \<Gamma>"
+        unfolding \<M>_prop_deci_def fset_of_list_simps fimage_finsert prod.sel
+      proof (rule minus_pfsubset_minusI)
+        show "fst |`| fset_of_list \<Gamma> |\<subset>| finsert (L \<cdot>l \<gamma>) (fst |`| fset_of_list \<Gamma>)"
+          using \<open>\<not> trail_defined_lit \<Gamma> (L \<cdot>l \<gamma>)\<close>[unfolded trail_defined_lit_def]
+          by (metis (no_types, lifting) finsertCI fset_of_list_elem fset_of_list_map
+              fsubset_finsertI list.set_map nless_le)
       next
-        have "L \<cdot>l \<gamma> \<in> {L \<in> \<Union> (ground_lits_of_lit ` \<Union> (set_mset ` fset N)). atm_of L \<prec>\<^sub>B \<beta>}"
-          unfolding mem_Collect_eq
-          using decideI
-          by (auto simp add: ground_lits_of_lit_def)
-        moreover have "fst ` set \<Gamma> \<subseteq>
-          {L \<in> \<Union> (ground_lits_of_lit ` \<Union> (set_mset ` fset N)). atm_of L \<prec>\<^sub>B \<beta>}"
-        proof (rule Set.subsetI, unfold mem_Collect_eq, rule conjI)
-          show "\<And>x. x \<in> fst ` set \<Gamma> \<Longrightarrow> atm_of x \<prec>\<^sub>B \<beta>"
-            using \<open>trail_atoms_lt \<beta> S'\<close>
-            by (auto simp add: trail_atoms_lt_def decideI(1))
-        next
-          fix K
-          show "K \<in> fst ` set \<Gamma> \<Longrightarrow> K \<in> \<Union> (ground_lits_of_lit ` \<Union> (set_mset ` fset N))"
-            using \<open>trail_lits_from_init_clauses N S'\<close>[unfolded trail_lits_from_init_clauses_def, rule_format, of K]
-            using \<open>trail_lits_ground S'\<close>[unfolded trail_lits_ground_def, rule_format, of K]
-            unfolding decideI(1,2) state_proj_simp
-            by (smt (verit, best) UN_absorb UnI1 generalizes_lit_def ground_lits_of_lit_def
-                mem_Collect_eq)
-        qed
-        ultimately show "fst ` set ((L \<cdot>l \<gamma>, None) # \<Gamma>) \<subseteq>
-          {L \<in> \<Union> (ground_lits_of_lit ` \<Union> (set_mset ` fset N)). atm_of L \<prec>\<^sub>B \<beta>}"
+        have "L \<cdot>l \<gamma> \<in> {L. atm_of L \<prec>\<^sub>B \<beta>}"
+          using \<open>atm_of L \<cdot>a \<gamma> \<prec>\<^sub>B \<beta>\<close>
           by simp
+        moreover have "fst ` set \<Gamma> \<subseteq> {L. atm_of L \<prec>\<^sub>B \<beta>}"
+          using \<open>trail_atoms_lt \<beta> S'\<close>
+          by (auto simp: trail_atoms_lt_def decideI(1))
+        ultimately have "insert (L \<cdot>l \<gamma>) (fst ` set \<Gamma>) \<subseteq> {L. atm_of L \<prec>\<^sub>B \<beta>}"
+          by simp
+        also have "\<dots> \<subseteq> {L. atm_of L \<prec>\<^sub>B \<beta> \<or> atm_of L = \<beta>}"
+          by blast
+        finally show "finsert (L \<cdot>l \<gamma>) (fst |`| fset_of_list \<Gamma>) |\<subseteq>|
+          Abs_fset {L. atm_of L \<prec>\<^sub>B \<beta> \<or> atm_of L = \<beta>}"
+          using finite_lits_less_eq_B
+          by (simp add: less_eq_fset.rep_eq fimage.rep_eq fset_of_list.rep_eq Abs_fset_inverse)
       qed
+      then show ?thesis
+        unfolding decideI(1,2) trail_decide_def \<M>_def state_proj_simp option.case
+        unfolding lex_prodp_def prod.sel by simp
     qed
   next
     assume "propagate N \<beta> S' S"
-    thus "\<M> N \<beta> S \<subset> \<M> N \<beta> S'"
+    thus "?less (\<M> N \<beta> S) (\<M> N \<beta> S')"
     proof (cases N \<beta> S' S rule: propagate.cases)
       case (propagateI C U L C' \<gamma> C\<^sub>0 C\<^sub>1 \<Gamma> \<mu> \<gamma>' \<rho> \<gamma>\<^sub>\<rho>')
 
@@ -227,154 +354,71 @@ proof (rule wfP_if_measurable)
       finally have "L \<cdot>l \<mu> \<cdot>l \<rho> \<cdot>l \<gamma>\<^sub>\<rho>' = L \<cdot>l \<gamma>"
         by assumption
 
-      show ?thesis
-        unfolding propagateI(1,2) trail_propagate_def \<M>.simps list.set image_insert prod.sel
-      proof (rule minus_psubset_minusI)
-        show "fst ` set \<Gamma> \<subset> insert (L \<cdot>l \<mu> \<cdot>l \<rho> \<cdot>l \<gamma>\<^sub>\<rho>') (fst ` set \<Gamma>)"
-          unfolding \<open>L \<cdot>l \<mu> \<cdot>l \<rho> \<cdot>l \<gamma>\<^sub>\<rho>' = L \<cdot>l \<gamma>\<close>
-          using \<open>\<not> trail_defined_lit \<Gamma> (L \<cdot>l \<gamma>)\<close>
-          by (metis insertCI psubsetI subset_insertI trail_defined_lit_def)
+      have "\<M>_prop_deci \<beta> ((L \<cdot>l \<gamma>, Some (C\<^sub>0 \<cdot> \<mu> \<cdot> \<rho>, L \<cdot>l \<mu> \<cdot>l \<rho>, \<gamma>\<^sub>\<rho>')) # \<Gamma>) |\<subset>| \<M>_prop_deci \<beta> \<Gamma>"
+        unfolding \<M>_prop_deci_def fset_of_list_simps fimage_finsert prod.sel
+      proof (rule minus_pfsubset_minusI)
+        show "fst |`| fset_of_list \<Gamma> |\<subset>| finsert (L \<cdot>l \<gamma>) (fst |`| fset_of_list \<Gamma>)"
+          using \<open>\<not> trail_defined_lit \<Gamma> (L \<cdot>l \<gamma>)\<close>[unfolded trail_defined_lit_def]
+          by (metis (no_types, lifting) finsertCI fset_of_list_elem fset_of_list_map
+              fsubset_finsertI list.set_map nless_le)
       next
-        show "insert (L \<cdot>l \<mu> \<cdot>l \<rho> \<cdot>l \<gamma>\<^sub>\<rho>') (fst ` set \<Gamma>) \<subseteq>
-          {L \<in> \<Union> (ground_lits_of_lit ` \<Union> (set_mset ` fset N)). atm_of L \<prec>\<^sub>B \<beta>}"
-          unfolding \<open>L \<cdot>l \<mu> \<cdot>l \<rho> \<cdot>l \<gamma>\<^sub>\<rho>' = L \<cdot>l \<gamma>\<close>
-        proof (intro Set.subsetI Set.CollectI conjI)
+        have "insert (L \<cdot>l \<gamma>) (fst ` set \<Gamma>) \<subseteq> {L. atm_of L \<prec>\<^sub>B \<beta>}"
+        proof (intro Set.subsetI Set.CollectI)
           fix K assume "K \<in> insert (L \<cdot>l \<gamma>) (fst ` set \<Gamma>)"
           thus "atm_of K \<prec>\<^sub>B \<beta>"
             using \<open>trail_atoms_lt \<beta> S'\<close>
             by (metis image_eqI insert_iff propagateI(1,4,6) state_trail_simp subst_cls_add_mset
                 trail_atoms_lt_def union_single_eq_member)
-        next
-          fix K assume K_in: "K \<in> insert (L \<cdot>l \<gamma>) (fst ` set \<Gamma>)"
-
-          from K_in have "is_ground_lit K"
-            using \<open>trail_lits_ground S'\<close>
-            by (metis insert_iff is_ground_cls_def propagateI(1,4,5) state_trail_simp
-                subst_cls_add_mset trail_lits_ground_def union_single_eq_member)
-
-          moreover from K_in have "\<exists>K'\<in>\<Union> (set_mset ` (fset N)). generalizes_lit K' K"
-            using \<open>trail_lits_from_init_clauses N S\<close>
-            unfolding trail_lits_from_init_clauses_def propagateI(1,2) trail_propagate_def \<open>L \<cdot>l \<mu> \<cdot>l \<rho> \<cdot>l \<gamma>\<^sub>\<rho>' = L \<cdot>l \<gamma>\<close>
-            unfolding state_proj_simp list.set image_insert prod.sel
-            by fast
-
-          ultimately show "K \<in> \<Union> (ground_lits_of_lit ` \<Union> (set_mset ` fset N))"
-            unfolding UN_iff
-            using \<open>trail_lits_from_init_clauses N S'\<close>[unfolded trail_lits_from_init_clauses_def propagateI(1,2) state_proj_simp]
-            by (smt (verit, best) ground_lits_of_lit_def mem_Collect_eq generalizes_lit_def)
         qed
+        also have "\<dots> \<subseteq> {L. atm_of L \<prec>\<^sub>B \<beta> \<or> atm_of L = \<beta>}"
+          by blast
+        finally show "finsert (L \<cdot>l \<gamma>) (fst |`| fset_of_list \<Gamma>) |\<subseteq>|
+          Abs_fset {L. atm_of L \<prec>\<^sub>B \<beta> \<or> atm_of L = \<beta>}"
+          using finite_lits_less_eq_B
+          by (simp add: less_eq_fset.rep_eq fimage.rep_eq fset_of_list.rep_eq Abs_fset_inverse)
       qed
+      thus ?thesis
+        unfolding propagateI(1,2) trail_propagate_def \<M>_def state_proj_simp option.case
+        unfolding \<open>L \<cdot>l \<mu> \<cdot>l \<rho> \<cdot>l \<gamma>\<^sub>\<rho>' = L \<cdot>l \<gamma>\<close>
+        unfolding lex_prodp_def prod.sel by simp
     qed
   next
-    show "conflict N \<beta> S' S \<Longrightarrow> \<M> N \<beta> S \<subset> \<M> N \<beta> S'" sorry
+    assume "conflict N \<beta> S' S"
+    thus "?less (\<M> N \<beta> S) (\<M> N \<beta> S')"
+    proof (cases N \<beta> S' S rule: conflict.cases)
+      case (conflictI D U \<gamma> \<Gamma> \<rho> \<gamma>\<^sub>\<rho>)
+      have "\<And>L. L |\<in>| fst |`| fset_of_list \<Gamma> \<Longrightarrow> atm_of L \<prec>\<^sub>B \<beta>"
+        using \<open>trail_atoms_lt \<beta> S'\<close>[unfolded conflictI(1,2) trail_atoms_lt_def, simplified]
+        by (metis (no_types, opaque_lifting) fimageE fset_of_list_elem)
+      hence "Pos \<beta> |\<notin>| fst |`| fset_of_list \<Gamma> \<and> Neg \<beta> |\<notin>| fst |`| fset_of_list \<Gamma>"
+        by (metis irreflpD irreflp_less_B literal.sel(1) literal.sel(2))
+      hence "finsert (Pos \<beta>) (finsert (Neg \<beta>) (Abs_fset {L. atm_of L \<prec>\<^sub>B \<beta>})) |-|
+        fst |`| fset_of_list \<Gamma> =
+        finsert (Pos \<beta>) (finsert (Neg \<beta>) (Abs_fset {L. atm_of L \<prec>\<^sub>B \<beta>} - fst |`| fset_of_list \<Gamma>))"
+        by (simp add: finsert_fminus_if)
+      hence "{||} |\<subset>| finsert (Pos \<beta>) (finsert (Neg \<beta>) (Abs_fset {L. atm_of L \<prec>\<^sub>B \<beta>})) |-| fst |`| fset_of_list \<Gamma>"
+        by auto
+      also have "\<dots> = \<M>_prop_deci \<beta> \<Gamma>"
+        unfolding \<M>_prop_deci_def
+        unfolding lits_less_eq_B_conv
+        using finite_lits_less_B
+        by (simp add: finsert_Abs_fset)
+      finally show ?thesis
+        unfolding lex_prodp_def conflictI(1,2)
+        unfolding \<M>_def state_proj_simp option.case prod.case prod.sel
+        by simp
+    qed
   next
-    show "skip N \<beta> S' S \<Longrightarrow> \<M> N \<beta> S \<subset> \<M> N \<beta> S'" sorry
+    show "skip N \<beta> S' S \<Longrightarrow> ?less (\<M> N \<beta> S) (\<M> N \<beta> S')" sorry
   next
-    show "factorize N \<beta> S' S \<Longrightarrow> \<M> N \<beta> S \<subset> \<M> N \<beta> S'" sorry
+    show "factorize N \<beta> S' S \<Longrightarrow> ?less (\<M> N \<beta> S) (\<M> N \<beta> S')" sorry
   next
-    show "resolve N \<beta> S' S \<Longrightarrow> \<M> N \<beta> S \<subset> \<M> N \<beta> S'" sorry
+    show "resolve N \<beta> S' S \<Longrightarrow> ?less (\<M> N \<beta> S) (\<M> N \<beta> S')" sorry
   qed
 next
-  show "wfP (\<subset>)"
-    oops
-
-
-
-
-
-
-
-
-
-
-
-
-thm scl_def reasonable_scl_def regular_scl_def
-
-definition regular_state ::
-  "('f, 'v) term clause set \<Rightarrow> ('f, 'v) term \<Rightarrow> ('f, 'v) state \<Rightarrow> bool" where
-  "regular_state N \<beta> S \<longleftrightarrow> True"
-
-definition regular ::
-  "_ \<Rightarrow> ('f, 'v) term clause set \<Rightarrow> ('f, 'v) term \<Rightarrow> _ \<Rightarrow> _ \<Rightarrow> bool"  where
-  "regular step N \<beta> S S' \<longleftrightarrow> regular_state N \<beta> S \<and> step N \<beta> S S'"
-
-definition reg_backtrack where
-  "reg_backtrack N \<beta> S S' \<longleftrightarrow> backtrack N \<beta> S S' \<and> (\<nexists>S''. conflict N \<beta> S S'')"
-
-thm wf_bounded_measure[of r ub f]
-
-term "conversep"
-
-lemma
-  assumes
-    "wfP R" and
-    "\<And>x y. (propagate N \<beta> \<squnion> decide N \<beta> \<squnion> conflict N \<beta> \<squnion> skip N \<beta> \<squnion>
-      factorize N \<beta> \<squnion> resolve N \<beta>)\<inverse>\<inverse> x y \<Longrightarrow> R (m\<^sub>R x) (m\<^sub>R y)"
-  shows "wfP (propagate N \<beta> \<squnion> decide N \<beta> \<squnion> conflict N \<beta> \<squnion> skip N \<beta> \<squnion> factorize N \<beta> \<squnion> resolve N \<beta> \<squnion>
-    backtrack N \<beta>)\<inverse>\<inverse>"
-proof -
-  define gnd_\<beta> where
-    "gnd_\<beta> \<equiv> {}"
-  define count_remaining :: "('f, 'v) state \<Rightarrow> nat" where
-    "count_remaining \<equiv> \<lambda>S. card gnd_\<beta> - card (state_learned S)"
-
-  show ?thesis
-    unfolding converse_join
-  proof (rule wfP_union_if_measurable)
-    show "wfP R"
-      by (rule assms(1))
-  next
-    fix S S' :: "('f, 'v) state"
-    show "((propagate N \<beta>)\<inverse>\<inverse> \<squnion> (decide N \<beta>)\<inverse>\<inverse> \<squnion> (conflict N \<beta>)\<inverse>\<inverse> \<squnion> (skip N \<beta>)\<inverse>\<inverse> \<squnion>
-      (factorize N \<beta>)\<inverse>\<inverse> \<squnion> (resolve N \<beta>)\<inverse>\<inverse>) S S' \<Longrightarrow> R (m\<^sub>R S) (m\<^sub>R S')"
-      by (rule assms(2)[unfolded converse_join])
-  next
-    show "wfP ((<) :: nat \<Rightarrow> nat \<Rightarrow> bool)"
-      by simp
-  next
-    fix S' S :: "('f, 'v) state" assume "(backtrack N \<beta>)\<inverse>\<inverse> S' S"
-    hence "backtrack N \<beta> S S'"
-      by simp
-    thus "count_remaining S' < count_remaining S"
-    proof (cases N \<beta> S S' rule: backtrack.cases)
-      case (backtrackI \<Gamma> \<Gamma>' \<Gamma>'' L \<sigma> D U)
-      then have "card (state_learned S') = Suc (card (state_learned S))"
-        sorry
-      moreover have "card gnd_\<beta> > card (state_learned S)"
-        sorry
-      ultimately show ?thesis
-        unfolding count_remaining_def by simp
-    qed
-  next
-    fix S' S :: "('f, 'v) state"
-    assume "((propagate N \<beta>)\<inverse>\<inverse> \<squnion> (decide N \<beta>)\<inverse>\<inverse> \<squnion> (conflict N \<beta>)\<inverse>\<inverse> \<squnion> (skip N \<beta>)\<inverse>\<inverse> \<squnion>
-      (factorize N \<beta>)\<inverse>\<inverse> \<squnion> (resolve N \<beta>)\<inverse>\<inverse>) S' S"
-    moreover have "propagate N \<beta> S S' \<Longrightarrow> state_learned S' = state_learned S"
-      by (erule propagate.cases) simp
-    moreover have "decide N \<beta> S S' \<Longrightarrow> state_learned S' = state_learned S"
-      by (erule decide.cases) simp
-    moreover have "conflict N \<beta> S S' \<Longrightarrow> state_learned S' = state_learned S"
-      by (erule conflict.cases) simp
-    moreover have "skip N \<beta> S S' \<Longrightarrow> state_learned S' = state_learned S"
-      by (erule skip.cases) simp
-    moreover have "factorize N \<beta> S S' \<Longrightarrow> state_learned S' = state_learned S"
-      by (erule factorize.cases) simp
-    moreover have "resolve N \<beta> S S' \<Longrightarrow> state_learned S' = state_learned S"
-      by (erule resolve.cases) simp
-    ultimately have "state_learned S' = state_learned S"
-      unfolding sup_apply sup_bool_def by (elim disjE) simp_all
-    thus "count_remaining S' < count_remaining S \<or> count_remaining S' = count_remaining S"
-      by (simp add: count_remaining_def)
-  qed
+  show "wfP (lex_prodp (|\<subset>|) (\<lambda>x y. (x, y) \<in> List.lenlex {(x :: nat, y :: nat). x < y}))"
+    by (rule wfP_lex_prodp) (simp_all add: wfP_pfsubset wfP_wf_eq wf_less wf_lenlex)
 qed
-
-lemma "wfP (scl N \<beta>)"
-proof -
-  show ?thesis
-  unfolding scl_def
-
-thm wfP_union_if_measurable
 
 
 end
